examples/elliptic/arm/mlton/bsubstML.sml
@@ -1,0 +1,85 @@
+structure bsubstML :> bsubstML =
+struct
+  nonfix empty_memory MEM_ITEMS MEM_WRITE_BLOCK MEM_WRITE MEM_WRITE_WORD
+         MEM_WRITE_BYTE MEM_READ SET_BYTE ADDR30 ::- :- * / div mod + -
+         ^ @ <> > < >= <= := o before;
+  
+  open numML fcpML wordsML;
+  type mem = (word30, word32) Redblackmap.dict
+  val mem_updates = ref ([]: word30 list)
+  fun :- a b = fn m => fn c => if a = c then b else m c
+    
+  fun ::- a l =
+        fn m => fn b =>
+        if word_ls a b andalso < (- (w2n b) (w2n a)) (listML.LENGTH l)
+          then listML.EL (- (w2n b) (w2n a)) l else m b
+    
+  fun ADDR30 addr =
+        word_extract_itself (Tyop ("i30", [])) (fromString"31") TWO addr
+    
+  fun SET_BYTE oareg b w =
+        word_modify (fn i => fn x =>
+          < i (fromString"8")
+          andalso
+          (if word_eq oareg (n2w_itself (ZERO,(Tyop ("i2", []))))
+             then index b i else x)
+          orelse
+          ((<= (fromString"8") i andalso < i (fromString"16"))
+           andalso
+           (if word_eq oareg (n2w_itself (ONE,(Tyop ("i2", []))))
+              then index b (- i (fromString"8")) else x)
+           orelse
+           ((<= (fromString"16") i andalso < i (fromString"24"))
+            andalso
+            (if word_eq oareg (n2w_itself (TWO,(Tyop ("i2", []))))
+               then index b (- i (fromString"16")) else x)
+            orelse
+            (<= (fromString"24") i andalso < i (fromString"32"))
+            andalso
+            (if word_eq oareg
+                  (n2w_itself ((fromString"3"),(Tyop ("i2", []))))
+               then index b (- i (fromString"24")) else x)))) w
+    
+  fun fromHexNum s n =
+        wordsML.fromNum(numML.fromHexString n, fcpML.Tyop (s, []));
+
+  val fromNum32 = (fromHexNum "i32"): string -> word32;
+
+  fun MEM_READ(m,a) = Redblackmap.find(m, a)
+                       handle NotFound => fromNum32 "E6000010";
+    
+  fun MEM_WRITE_BYTE mem addr word =
+        let val addr30 = ADDR30 addr
+        in
+           Redblackmap.insert(mem, (addr30: word30),
+             SET_BYTE
+                (word_extract_itself (Tyop ("i2", [])) ONE ZERO addr)
+                (word_extract_itself (Tyop ("i8", [])) (fromString"7")
+                   ZERO word) (MEM_READ(mem,addr30)))
+        end
+
+  fun MEM_WRITE_WORD (mem:mem) addr word =
+        Redblackmap.insert(mem,ADDR30 addr,word)
+
+  fun MEM_WRITE b m a =
+        (:= (mem_updates, ADDR30 a :: !mem_updates);
+          if b then MEM_WRITE_BYTE m a else MEM_WRITE_WORD m a)
+
+  fun MEM_WRITE_BLOCK m (a: word30) [] = m
+    | MEM_WRITE_BLOCK m a (d::l) =
+       (:= (mem_updates, ADDR30 a :: !mem_updates);
+        MEM_WRITE_BLOCK (Redblackmap.insert(m, a, (d: word32)))
+          (word_add a (n2w_itself (ONE,(Tyop ("i30", []))))) l)
+    
+  fun MEM_ITEMS (m:mem) = Redblackmap.listItems m
+
+  fun word_compare(v, w) =
+    let val m = w2n v and n = w2n w in
+      if m = n then
+        EQUAL
+      else
+        if < m n then LESS else GREATER
+    end
+
+  val empty_memory = (Redblackmap.mkDict word_compare):mem
+end
