examples/elliptic/arm/arm_rulesScript.sml
@@ -12,7 +12,7 @@
 
 open HolKernel boolLib Parse bossLib;
 open Q arithmeticTheory bitTheory wordsTheory wordsLib;
-open armTheory arm_evalTheory;
+open bsubstTheory armTheory arm_evalTheory;
 
 val _ = new_theory "arm_rules";
 
